\documentclass{article}
 
\usepackage{geometry} 
\geometry{
	a4paper,
	total={170mm, 257mm},
	left=20mm,
	top=20mm,
}

\usepackage[fleqn]{amsmath}
\setlength\parindent{0pt}
 


\begin{document}
	
	
	\begin{center}
		\section*{WPG}
		{\Large Practical \LaTeX\, Tutorial \# 24}
	\end{center}	
	\section*{Mathematics Formulas and Algebraic Equations}
	 
	\hrule
	\bigskip
	\bigskip
	\bigskip
	
	\section{Mathematics Formulas and Algebraic Equations}
	
	\subsection{Function Relationships}
	\begin{align*}
		\sin{\theta} &= \frac{1}{\csc{\theta}}\\
		\cos{\theta} &= \frac{1}{\sec{\theta}}\\
		\tan{\theta} &= \frac{1}{\cot{\theta}}\\
		\csc{\theta} &= \frac{\sin{\theta}}{\cos{\theta}}\\
		\sec{\theta} &= \frac{1}{\cos{\theta}}\\
		\cot{\theta} &= \frac{1}{\tan{\theta}}\\
		\cot{\theta} &= \frac{\cos{\theta}}{\sin{\theta}}
	\end{align*}
	
	
	\subsection{Opposite Angle Formulas}	
	\begin{align*}
		\sin{(-\theta)} &= -\sin{(-\theta)}\\
		\cos{(-\theta)} &= -\cos{(\theta)}\\		
		\tan{(-\theta)} &= -\tan{(\theta)}\\
		\cot{(-\theta)} &= -\cot{(\theta)}\\
		\sec{(-\theta)} &= -\sin{(\theta)}\\		
		\csc{(-\theta)} &= -\csc{(\theta)}
	\end{align*}
	
	
	\subsection{Confusion Formulas (in Quadrant I)}
	\begin{align*}
		\sin{\theta} &= \cos{\left( \frac{\pi}{2} - \theta  \right)}\\
		\tan{\theta} &= \cot{\left( \frac{\pi}{2} - \theta  \right)}\\
		\sec{\theta} &= \csc{\left( \frac{\pi}{2} - \theta  \right)}\\		
		\cos{\theta} &= \sin{\left( \frac{\pi}{2} - \theta  \right)}\\
		\cot{\theta} &= \tan{\left( \frac{\pi}{2} - \theta  \right)}\\
		\csc{\theta} &= \sec{\left( \frac{\pi}{2} - \theta  \right)}
	\end{align*}
	
	
	\subsection{Pythagorean Identities}
	\begin{align*}
		\sin^2{\theta} + \cos^2{\theta} = 1\\
		\tan^2{\theta} + 1 = \sec^2{\theta} \\
		\cot^2{\theta} + 1 = \csc^2{\theta}
	\end{align*}
	
	
	
	\subsection{Half Angle Formulas}
	\begin{align*}
		\sin{\frac{\theta}{2}} &= \pm \sqrt{\frac{1 - \cos{\theta}}{2}}\\
		\cos{\frac{\theta}{2}} &= \pm \sqrt{\frac{1 + \cos{\theta}}{2}}\\
		\tan{\frac{\theta}{2}} &= \pm \sqrt{\frac{1 - \cos{\theta}}{1 + \cos{\theta}}}\\
								&= \frac{1-\cos{\theta}}{\sin{\theta}} \\
								&= \frac{\sin{\theta}}{1 + \cos{\theta}}
	\end{align*}
	
	
	\subsection{Double Angle Formulas}
	\begin{align*}
		\sin{2\theta} &= 2 \sin{\theta} \cos{\theta}\\
		\cos{2\theta} &= \cos^2{\theta} - \sin^2{\theta} \\
						&= 1 - 2 \sin^2{\theta} \\
						&= 2 \cos^2{\theta} - 1 \\
		\tan{2\theta} &= \dfrac{2\tan{\theta}}{1 - \tan^2{\theta}}
	\end{align*}
	
	
	
	\subsection{Triple Angle Formulas}		
	\begin{align*}
		\sin{3\theta} &= 3\sin{\theta} - 4 \sin^3{\theta} \\
		\cos{3\theta} &= 4 \cos^3{\theta} - 3\cos{\theta} \\
		\tan{3\theta} &= \dfrac{3\tan{\theta} - \tan^3{\theta}}{1 - 3 \tan^2{\theta}}
	\end{align*}
	
	
	\subsection{Angle Addition Formulas}	
	\begin{align*}
		\sin{(A + B)} &= \sin{A} \cos{B} + \cos{A}\sin{B}\\
		\sin{(A - B)} &= \sin{A} \cos{B} - \cos{A}\sin{B}\\
		\cos{(A + B)} &= \cos{A} \cos{B} - \sin{A}\sin{B}\\
		\cos{(A - B)} &= \sin{A} \cos{B} + \sin{A}\sin{B}\\		
		\tan{(A + B)} &= \dfrac{\tan{A} + \tan{B}}{1 - \tan{A}\tan{B}}\\
		\tan{(A - B)} &= \dfrac{\tan{A} - \tan{B}}{1 + \tan{A}\tan{B}}
	\end{align*}
	
	
	
	
	\subsection{Power Reducing Formulas}
	\begin{align*}
		\sin^2{\theta} &= \dfrac{1 - \cos{2\theta}}{2}\\
		\cos^2{\theta} &= \dfrac{1 + \cos{2\theta}}{2}\\
		\tan^2{\theta} &= \dfrac{1 - \cos{2\theta}}{1 + \cos{2\theta}}
	\end{align*}
	
	
	\subsection{Product-to-Sum Formulas}	
	\begin{align*}
		\sin{A} \cdot \sin{B} &= \dfrac{1}{2} \left[ \cos{(A - B)} - \cos{A + B}  \right]\\
		\cos{A} \cdot \cos{B} &= \dfrac{1}{2} \left[ \cos{(A - B)} + \cos{A + B}  \right]\\
		\sin{A} \cdot \cos{B} &= \dfrac{1}{2} \left[ \sin{(A - B)} + \sin{A + B}  \right]\\
		\cos{A} \cdot \sin{B} &= \dfrac{1}{2} \left[ \sin{(A + B)} - \sin{A - B}  \right]
	\end{align*}
	
	
	\subsection{Sum-to-Product Formulas}
	\begin{align*}
		\sin{A} + \sin{B} &= 2 \cdot \sin{\left( \dfrac{A + B}{2}  \right)} \cdot \cos{\left( \dfrac{A - B}{2}  \right)}\\
		\sin{A} - \sin{B} &= 2 \cdot \sin{\left( \dfrac{A - B}{2}  \right)} \cdot \cos{\left( \dfrac{A + B}{2}  \right)}\\
		\cos{A} + \cos{B} &= 2 \cdot \cos{\left( \dfrac{A + B}{2}  \right)} \cdot \cos{\left( \dfrac{A + B}{2}  \right)}\\
		\cos{A} - \cos{B} &= 2 \cdot \sin{\left( \dfrac{A + B}{2}  \right)} \cdot \cos{\left( \dfrac{A - B}{2}  \right)}
	\end{align*}
	
	
	\subsection{Arc Length}
	$S = r\theta$
	
	
	\subsection{Law of Sines}
	$\dfrac{a}{\sin{A}} = \dfrac{b}{\sin{B}} = \dfrac{c}{\sin{C}}$
	
	
	\subsection{Law of Cosines}
	\begin{align*}
		a^2 &= b^2 + c^2 - 2bc \cos{A} \\
		b^2 &= a^2 + c^2 - 2ac \cos{B} \\
		c^2 &= a^2 + b^2 - 2ab \cos{C}
	\end{align*}
	
	
	\subsection{Law of Tangents}
	$\dfrac{a - b}{a + b} = \dfrac{\tan{\left[ \dfrac{1}{2}(A - B)  \right]}}{\tan{\left[ \dfrac{1}{2}(A + B)  \right]}}$
	
	
	\subsection{Euler's Formula}
	$e^{i\theta} = \cos{\theta} + i\sin{\theta}$
	
	
	\subsection{Polar Multiplication and Division}
	\par Let: \quad $a = r_1 cis \theta$ \quad $b = r_2 cis \rho$\\[3ex]
	$a \cdot b = r_1r_2 cis (\theta + \rho) \quad \dfrac{a}{b} = \dfrac{r_1}{r_2} cis (\theta - \rho)$
	
	
	\subsection{Mollweide's Formulas}	
	\begin{align*}
		\dfrac{a - b}{c} &= \dfrac{\cos{\left[ \dfrac{1}{2}(A - B) \right]}}{\sin{\left(  \dfrac{1}{2} C\right)}}\\
		\dfrac{a - b}{c} &= \dfrac{\sin{\left[ \dfrac{1}{2}(A - B) \right]}}{\cos{\left(  \dfrac{1}{2} C\right)}}
	\end{align*}
	
	
	
	
	
	
	
	
	
	
	
	
	
	
	
	
	
	
	
	
	
	
	
	
	
	
	
	
	
	
	
	
	
	
	
	

\end{document}