\documentclass{article}
 
\usepackage{amsmath}
\usepackage{mathtools}
\usepackage{geometry}
\geometry{
	a4paper,
	total={170mm,257mm},
	left=20mm,
	top=20mm,
}

\setlength\parindent{0pt}


\begin{document}
	
	
	\begin{center}
		\section*{WPG}
		{\Large Practical \LaTeX\, Tutorial \# 23}
	\end{center}	
	\subsection*{Objectives}
	\begin{itemize}
		\item Aligned Formulas
		\item Cases Environment
		\item Example
	\end{itemize}
	\hrule
	\bigskip
	
	
	
	\section*{Cases Environment}
	
	$$
	\vert x \vert = \begin{cases}
			x, 			& \text{x $\ge 0$}\\
			-x, 		& \text{x $< 0$}
		\end{cases}
	$$
	
	$$
	f(x) = \begin{cases}
			0, 				& \text{x $\le -1$}\\
			\sqrt{1-x^2}, 	& \text{$-1 < $ x $< 1$}\\
			x,				& \text{x $\ge 1$}
		\end{cases}
	$$
	
	
	\begin{align*} 
		\vert x \vert &= \begin{cases}
			x, 			& \text{x $\ge 0$}\\
			-x, 		& \text{x $< 0$}
			\end{cases}\\	
		f(x) &= \begin{cases}
				0,		 		& \text{x $\le -1$}\\
				\sqrt{1-x^2}, 	& \text{$-1 < $ x $< 1$}\\
				x, 				& \text{x $\ge 1$}
			\end{cases}  
	\end{align*}
	
	

	$$
		\lim_{x\to 2-} f(x) = 6, \text{where} f(x) = \begin{cases}
										x, 			& \text{$x>2$}\\
										3x, 		& \text{$x \le 2$}
									\end{cases}
	$$
	
	
	
	
	
	
	\begin{align*}
	V_{ijk} = \begin{cases}
		\dfrac{y_u +y_t}{2} - \dfrac{x_u+x_t}{2}, 			& \text{if $x_u < y_t$}\\[4ex]
		\begin{multlined}
			\dfrac{1}{C} \biggl[ \dfrac{x_u^3 - y_u^3}{6} + \dfrac{y_t^2 + x_u^2}{2} x_l + \left( x_u -y_t  \right)\dfrac{x_l^2}{2} \\
			+ \dfrac{y_u^2 - x_u^2}{x} \left( x_u - x_l \right)  - \left( y_u - x_u  \right) \dfrac{x_u^2 -x_t^2}{2}  \biggr] 	
		\end{multlined},  									& \text{if $x_u \in [y_t, y_u]$} \\[8ex]
		\dfrac{1}{x_u - x_l} \left[ \dfrac{(y_u + y_t)^2}{6} - \dfrac{y_u  + y_t}{2} x_l + \dfrac{x_l^2}{2}  \right], 					& \text{otherwise}
	\end{cases}
	\end{align*}
	
	
	
	
	
	
	
	
	
	
	
	
	
	
	
	
	
	
	
	
	
	
	
	
	
	
	
	
	
	
	
	
	
	
%	\begin{align*}
%		V_{ijk} = \begin{cases}
%			\dfrac{y_u + y_t}{2} - \dfrac{x_u + x_t}{2}, 		& \text{if $x_u < y_t$} \\[4ex]
%			\begin{multlined}
%				\dfrac{1}{C} \biggl[ \dfrac{x_u^3 - y_t^3}{6} + \dfrac{y_t^2 + x_u^2}{2}x_l + \left(x_u - y_t\right) \dfrac{x_l^2}{2}\\
%				 + \dfrac{y_u^2 - x_u^2}{2} \left( x_u - x_l \right) - \left( y_u - x_u \right) \dfrac{x_u^2 - x_t^2}{2}   \biggr]
%			\end{multlined}, 									& \text{if $x_u \in [y_t, y_u]$} \\[8ex]
%			\dfrac{1}{x_u - x_l}\left[ \dfrac{(y_u + y_t)^2}{6} - \dfrac{y_u + y_t}{2} x_l + \dfrac{x_l^2}{2} \right], 							& \text{otherwise}
%		\end{cases}
%	\end{align*}
	
	 

	

\end{document}